Refactors

AVLTree.fst
@@ -36,10 +36,10 @@ val is_bst : tree -> Tot bool
 let rec is_bst t =
   match t with
   | Leaf -> true
-  | Node n (t1, h1) (t2, h2) -> all (fun n' -> n > n') t1 &&
+  | Node n (t1, _) (t2, _) -> all (fun n' -> n > n') t1 &&
                     all (fun n' -> n < n') t2 && is_bst t1 && is_bst t2
 
-                   
+type bst = t:tree{is_bst t}                   
 
 val create_tree: n:int -> tree 
     -> tree -> Tot tree
@@ -63,6 +63,7 @@ val is_avl: t:tree -> Tot bool
 let is_avl t = 
     is_bst t && is_balanced t 
 
+type avl = t:tree{is_avl t}
                     
 val search : x:int -> t:tree{is_bst t} ->
   Tot (r:bool{r <==> in_tree x t})
@@ -73,12 +74,13 @@ let rec search x t =
                     else if x < n then search x t1
                     else               search x t2
 
-val insert_bst : x:int -> t:tree{is_bst t} ->
-  Tot (r:tree{is_bst r /\ (forall y. in_tree y r <==> (in_tree y t \/ x = y))})
+val insert_bst : x:int -> t:bst ->
+  Tot (r:bst{(forall y. in_tree y r <==> (in_tree y t \/ x = y))})
 let rec insert_bst x t =
   match t with
   | Leaf -> create_tree x Leaf Leaf
-  | Node n (t1, h1) (t2, h2) -> if x = n then      t
+  | Node n (t1, h1) (t2, h2) -> 
+					if x = n then      t
                     else if x < n then create_tree n (insert_bst x t1) t2
                     else               create_tree n t1 (insert_bst x t2)
 
@@ -94,7 +96,7 @@ let rec rebalance t =
             if bf tr <> -1 then t
             else t
   
-val insert_avl: x:int -> t:tree{is_balanced t} -> 
+val insert_avl: x:int -> t:avl -> 
   Tot (r:tree{ (forall y. in_tree y r <==> (in_tree y t \/ x = y))})
 
 let rec insert_avl x t = 
@@ -105,7 +107,7 @@ let rec insert_avl x t =
                     else               create_tree n t1 (insert_avl x t2))
 
 
-val left_rotate: t:tree{is_bst t}  -> Tot (r:tree{is_bst r})
+val left_rotate: t:bst  -> Tot (r:bst)
 let rec left_rotate t =
     match t with 
     |   Leaf -> Leaf  
@@ -116,19 +118,13 @@ let rec left_rotate t =
             create_tree y (create_tree x a_tree b_tree) c_tree
 
 
-
 val create_tree_keeps_elems: n:int -> t1:tree{is_bst t1} -> t2:tree{is_bst t2} ->
-    (Lemma(requires true)( ensures forall y. in_tree y (create_tree n t1 t2) <==> in_tree y t1  \/ in_tree y t2 \/ n = y  ) )
+    Lemma(forall y. in_tree y (create_tree n t1 t2) <==> in_tree y t1  \/ in_tree y t2 \/ n = y) 
 
 let rec create_tree_keeps_elems n t1 t2 = 
     ()
 
-val left_rotate_keeps_elements: t:tree{is_bst t} -> Lemma(requires true)(ensures (forall y. in_tree y (left_rotate t) <==> in_tree y t ) )
+val left_rotate_keeps_elements: t:bst -> Lemma(forall y. in_tree y (left_rotate t) <==> in_tree y t )
 
 let rec left_rotate_keeps_elements t =
-    match t with 
-    |   Leaf -> ()  
-    |   Node x (a_tree, _) (y_tree, h2) ->
-        match y_tree with
-        |   Leaf -> () 
-        |   Node y (b_tree, _) (c_tree, _) -> ()
+    ()
